finished proof of termination of mgu. Annotated mgu.fst

mgu.fst
@@ -5,12 +5,14 @@ open Subst
 open Fset
 open Union
 
+(** The function applies a substitution on a list of tuples of terms. **)
 val apply_tuple_list : st:subst -> l:list (term*term) -> Tot (list (term*term))
 
 let rec apply_tuple_list st l = match l with
   | [] -> []
   | (hd1,hd2)::tl -> (apply st hd1 , apply st hd2)::(apply_tuple_list st tl)
 
+(** States that the length of the list is unchanged on application of a substitution **)
 val apply_list_length_lemma : st:subst -> l:list (term*term) -> Lemma
   (requires true)
   (ensures ( List.Tot.length l = List.Tot.length (apply_tuple_list st l)) )
@@ -19,6 +21,7 @@ let rec apply_list_length_lemma st l = match l with
   | [] -> ()
   | hd::tl -> apply_list_length_lemma st tl
 
+(** This function joins 2 lists of terms and forms a list of tuples of terms. The lists have to be of equal length. **)
 val collate : l1:list term -> l2:list term {List.Tot.length l1 = List.Tot.length l2}-> Tot (list (term*term))
 
 let rec collate l1 l2 = match l1,l2 with
@@ -29,21 +32,7 @@ let rec collate l1 l2 = match l1,l2 with
 
 let rec is_Unifiable*)
 
-(*val get_list_of_vars : term -> list variable -> Tot (list variable)
-val get_list_of_vars_list : list term -> list variable -> Tot (list variable)
-
-let rec get_list_of_vars t lv =
-  match t with
-  | Var v -> if mem v lv then lv else v::lv
-  | Name n -> lv
-  | (Func s args) -> get_list_of_vars_list args lv
-and get_list_of_vars_list lt lv = match lt with
-  | [] -> lv
-  | hd::tl -> begin
-                let temp1 = get_list_of_vars hd lv in
-                get_list_of_vars_list tl temp1
-              end*)
-
+(** These functions return the set of variables in a term and in a list of term respectively. **)
 val get_fset_vars : term -> Tot (fset variable)
 val get_fset_vars_list : list term -> Tot (fset variable)
 
@@ -55,6 +44,7 @@ and get_fset_vars_list lt = match lt with
   | [] -> fempty
   | hd::tl -> funion (get_fset_vars hd) (get_fset_vars_list tl)
 
+(** These functions return the number of symbols in a term and in a list of terms. **)
 val get_num_symbols : t:term -> Tot nat
 val get_num_symbols_list : lt:list term-> Tot nat
 
@@ -67,18 +57,21 @@ and get_num_symbols_list lt = match lt with
   | [] -> 0
   | hd::tl -> get_num_symbols hd + get_num_symbols_list tl
 
+(** The function which returns the number of symbols in a list of tuples of terms **)
 val get_num_symbols_tuple_list : ltt:list (term*term) -> Tot nat
 
 let rec get_num_symbols_tuple_list ltt = match ltt with
   | [] -> 0
   | (hd1,hd2)::tl -> get_num_symbols hd1 + get_num_symbols hd2 + get_num_symbols_tuple_list tl
 
+(** The function which returns the set of variables in a list of tuples of terms **)
 val get_fset_vars_tuple_list : list (term*term) -> Tot (fset variable)
 
 let rec get_fset_vars_tuple_list ltt = match ltt with
   | [] -> fempty
   | (hd1,hd2)::tl -> funion (get_fset_vars hd1)  (funion (get_fset_vars hd2) (get_fset_vars_tuple_list tl))
 
+(** States that the set of variable in (t1,t2)::ltt is same as that of (t2,t1)::ltt **)
 val tuple_fset_lemma : t1:term -> t2:term -> ltt: list (term*term) -> Lemma
   (requires true)
   (ensures (equal (get_fset_vars_tuple_list ( (t1,t2)::ltt )) (get_fset_vars_tuple_list ( (t2,t1)::ltt ))) )
@@ -86,6 +79,7 @@ val tuple_fset_lemma : t1:term -> t2:term -> ltt: list (term*term) -> Lemma
 
 let tuple_fset_lemma t1 t2 ltt = ()
 
+(** Supporting lemmas for aux_lemma1c. State that vars(x{t/v}) is a subset of vars(x) U vars(t)  **)
 val aux_lemma1a : x:term -> v:variable -> t:term -> Lemma
   (requires not(is_var_present v t))
   (ensures fsubset (get_fset_vars (apply [(v,t)] x)) (funion (get_fset_vars x) (get_fset_vars t)) )
@@ -104,6 +98,7 @@ let rec aux_lemma1a x v t = match x with
   | [] -> ()
   | hd::tl -> aux_lemma1a hd v t; aux_lemma1b tl v t
 
+(** Supporting lemma for aux_lemma5. States that vars(ltt{t/v}) is a subset of vars( (Var v,t)::ltt ) **)
 val aux_lemma1c : ltt:list (term*term) -> v:variable -> t:term -> Lemma
   (requires not(is_var_present v t))
   (ensures fsubset (get_fset_vars_tuple_list (apply_tuple_list [(v,t)] ltt)) (get_fset_vars_tuple_list ( (Var v,t)::ltt ) ) )
@@ -112,12 +107,14 @@ let rec aux_lemma1c ltt v t = match ltt with
   | [] -> ()
   | (hd1,hd2)::tl -> aux_lemma1a hd1 v t; aux_lemma1a hd2 v t; aux_lemma1c tl v t
 
+  (** Supporting lemma for aux_lemma5. States that the variable v is present in the tuple list (Var v, t)::ltt **)
 val aux_lemma2 : ltt:list (term*term) -> v:variable -> t:term -> Lemma
   (requires true)
   (ensures (mem v (get_fset_vars_tuple_list ((Var v,t)::ltt))) )
 
 let aux_lemma2 ltt v t = ()
 
+(** Supporting lemma for aux_lemma5. States that if is_var_present v t is false then v isnt present in the set of variables. **)
 val aux_lemma3a : v:variable -> t:term -> Lemma (requires not(is_var_present v t)) (ensures not(mem v (get_fset_vars t)))
 val aux_lemma3b : v:variable -> lt:list term -> Lemma (requires not(is_var_present_list v lt)) (ensures not(mem v (get_fset_vars_list lt)))
 
@@ -129,6 +126,7 @@ and aux_lemma3b v lt = match lt with
   | [] -> ()
   | hd::tl -> aux_lemma3a v hd ; aux_lemma3b v tl
 
+(** Supporting lemma for aux_lemma5. States that the variable v is not present in the term after application of the substution {t/v} **)
 val aux_lemma4a : t:term -> v:variable -> x:term -> Lemma(requires not(is_var_present v x))(ensures not(mem v (get_fset_vars (apply [(v,x)] t) )))
 val aux_lemma4b : lt:list term -> v:variable -> x:term -> Lemma(requires not(is_var_present v x))(ensures not(mem v (get_fset_vars_list (apply_list [(v,x)] lt) )))
 
@@ -142,6 +140,7 @@ and aux_lemma4b lt v x = match lt with
   | [] -> ()
   | hd::tl -> aux_lemma4a hd v x ;  aux_lemma4b tl v x
 
+(** Supporting lemma for aux_lemma5. States that the variable v is not present in the set of variables of a list of tuple of terms after application of the substitution {t/v} **)
 val aux_lemma3 : ltt:list (term*term) -> v:variable -> t:term -> Lemma
   (requires not(is_var_present v t))
   (ensures not(mem v (get_fset_vars_tuple_list (apply_tuple_list [(v,t)] ltt))))
@@ -150,6 +149,7 @@ let rec aux_lemma3 ltt v t = match ltt with
   | [] -> ()
   | (hd1,hd2)::tl -> aux_lemma4a hd1 v t; aux_lemma4a hd2 v t; aux_lemma3 tl v t
 
+(** Lemma for proving termination in 1st case. States that the number of variables decreases from the first call to the second. **)
 val aux_lemma5 : ltt:list (term*term) -> v:variable -> t:term -> Lemma
   (requires not(is_var_present v t))
   (ensures size (get_fset_vars_tuple_list (apply_tuple_list [(v,t)] ltt)) < size (get_fset_vars_tuple_list ((Var v,t)::ltt)) )
@@ -157,16 +157,58 @@ val aux_lemma5 : ltt:list (term*term) -> v:variable -> t:term -> Lemma
 let rec aux_lemma5 ltt v t = aux_lemma1c ltt v t; aux_lemma2 ltt v t; aux_lemma3 ltt v t ;
                              size_lemma v (get_fset_vars_tuple_list (apply_tuple_list [(v,t)] ltt)) (get_fset_vars_tuple_list ((Var v,t)::ltt))
 
-assume val aux_lemma6 : lt1:list term -> lt2:list term {List.Tot.length lt2 = List.Tot.length lt1} ->  ltt:list (term*term) -> s:symbol { s.arity = List.Tot.length lt1} -> Lemma
+(** Supporting lemma for aux_lemma7. States that the set of variables in the concatenation of 2 lists is equal to the union of the sets of variables in the lists. **)
+val aux_lemma6a : ltt1:list (term*term) -> ltt2:list (term*term) -> Lemma
+  (requires true)
+  (ensures (equal (get_fset_vars_tuple_list (List.Tot.append ltt1 ltt2)) (funion (get_fset_vars_tuple_list ltt1) (get_fset_vars_tuple_list ltt2))))
+
+let rec aux_lemma6a ltt1 ltt2 = match ltt1 with
+  | [] -> ()
+  | hd::tl -> aux_lemma6a tl ltt2
+
+(** Supporting lemma for aux_lemma7. States that the set of variables in the collated form of 2 lists is equal to the union of the sets of variables of the 2 lists. **)
+val aux_lemma6b : lt1:list term -> lt2:list term { List.Tot.length lt2 = List.Tot.length lt1 } -> Lemma
+  (requires true)
+  (ensures (equal (get_fset_vars_tuple_list (collate lt1 lt2)) (funion (get_fset_vars_list lt1) (get_fset_vars_list lt2))))
+
+let rec aux_lemma6b lt1 lt2 = match lt1,lt2 with
+  | [],[] -> ()
+  | hd1::tl1,hd2::tl2 -> aux_lemma6b tl1 tl2
+
+(** Lemma for proving termination in the third case. States that the size of the variables set remains the same between the two calls. **)
+val aux_lemma7 : lt1:list term -> lt2:list term {List.Tot.length lt2 = List.Tot.length lt1} ->  ltt:list (term*term) -> s:symbol { s.arity = List.Tot.length lt1 } -> Lemma
   (requires true )
   (ensures ( size (get_fset_vars_tuple_list (List.Tot.append (collate lt1 lt2) ltt)) = size (get_fset_vars_tuple_list ((Func s lt1, Func s lt2)::ltt)) ) )
 
-assume val aux_lemma7 : lt1:list term -> lt2:list term {List.Tot.length lt2 = List.Tot.length lt1} ->  ltt:list (term*term) -> s:symbol { s.arity = List.Tot.length lt1} -> Lemma
+let rec aux_lemma7 lt1 lt2 ltt s = aux_lemma6a (collate lt1 lt2) ltt; aux_lemma6b lt1 lt2
+
+(** Supporting lemma for aux_lemma10. States that the number of symbols in the collated form of 2 lists is equal to the sum of the numbers of symbols in each of them **)
+val aux_lemma8 : lt1:list term -> lt2:list term { List.Tot.length lt2 = List.Tot.length lt1 } -> Lemma
+  (requires true)
+  (ensures (get_num_symbols_tuple_list (collate lt1 lt2) = get_num_symbols_list lt1 + get_num_symbols_list lt2))
+
+let rec aux_lemma8 lt1 lt2 = match lt1,lt2 with
+  | [],[] -> ()
+  | hd1::tl1,hd2::tl2 -> aux_lemma8 tl1 tl2
+
+(** Supporting lemma for aux_lemma10. States that the number of symbols in the concatenation of 2 lists is equal to the sum of the numbers of symbols in each of them **)
+val aux_lemma9 : ltt1:list (term*term) -> ltt2:list (term*term) -> Lemma
+  (requires true)
+  (ensures (get_num_symbols_tuple_list (List.Tot.append ltt1 ltt2) = get_num_symbols_tuple_list ltt1 + get_num_symbols_tuple_list ltt2))
+
+let rec aux_lemma9 ltt1 ltt2 = match ltt1 with
+  | [] -> ()
+  | hd::tl -> aux_lemma9 tl ltt2
+
+(** Lemma for proving termination in the third case. States that the number of symbols decreases. **)
+val aux_lemma10 : lt1:list term -> lt2:list term {List.Tot.length lt2 = List.Tot.length lt1} ->  ltt:list (term*term) -> s:symbol { s.arity = List.Tot.length lt1} -> Lemma
   (requires true )
-  (ensures ( get_num_symbols_tuple_list(List.Tot.append (collate lt1 lt2) ltt) < get_num_symbols_tuple_list((Func s lt1, Func s lt2)::ltt)) )
+  (ensures ( get_num_symbols_tuple_list (List.Tot.append (collate lt1 lt2) ltt) < get_num_symbols_tuple_list((Func s lt1, Func s lt2)::ltt)) )
 
-(*let rec aux_lemma6 lt1 lt2 ltt s =*)
+let rec aux_lemma10 lt1 lt2 ltt s = aux_lemma9 (collate lt1 lt2) ltt; aux_lemma8 lt1 lt2
 
+(** The main function calculating the mgu, takes in a list of tuple of terms and a substitution as an argument.
+The substitution represents the (var,term) pairs already covered in the list thus far. May or may not return a substitution. **)
 val sub_mgu : l:list (term*term) -> st:subst -> Tot (option subst) (decreases %[size (get_fset_vars_tuple_list l);(get_num_symbols_tuple_list l)])
 let rec sub_mgu l st = match l with
   | [] -> Some st
@@ -185,9 +227,10 @@ let rec sub_mgu l st = match l with
       assert(size (get_fset_vars_tuple_list tl) = size (get_fset_vars_tuple_list l));
       sub_mgu tl st
       ) else None
-  | (Func s1 args1, Func s2 args2)::tl -> if s1 = s2 then (aux_lemma6 args1 args2 tl s1; aux_lemma7 args1 args2 tl s1;  sub_mgu (List.Tot.append (collate args1 args2) tl) st) else None
+  | (Func s1 args1, Func s2 args2)::tl -> if s1 = s2 then (aux_lemma7 args1 args2 tl s1; aux_lemma10 args1 args2 tl s1;  sub_mgu (List.Tot.append (collate args1 args2) tl) st) else None
   | _ -> None
 
+  (** The main mgu function. Has a call to sub_mgu **)
 val mgu : l:list (term*term) -> Tot (option subst)
 
 let mgu l= sub_mgu l []
